commutation lemma proved

subst.fst
@@ -62,13 +62,13 @@ val apply : subst -> term ->Tot term
 val apply_list : subst -> l1:list term ->Tot (l2:list term{FStar.List.Tot.length l1 = FStar.List.Tot.length l2})
 
 (**Returns the term that the input variable corresponds to in the substitution**)
-val get_Term : v:variable -> s:subst{ mem v (get_Domain s) } -> Tot term
+val get_Image : v:variable -> s:subst{ mem v (get_Domain s) } -> Tot term
 
-let rec get_Term v st= match st with
-  | hd::tl -> if (fst hd)=v then (snd hd) else (get_Term v tl)
+let rec get_Image v st= match st with
+  | hd::tl -> if (fst hd)=v then (snd hd) else (get_Image v tl)
 
 let rec apply st t = match t with
-  | Var v -> if mem v (get_Domain st) then (get_Term v st) else t
+  | Var v -> if mem v (get_Domain st) then (get_Image v st) else t
   | Func s args -> Func s (apply_list st args)
   | Name n -> t
   and apply_list st lt = match lt with
@@ -98,12 +98,27 @@ let is_composable st1 st2 = (distinct_domain st1 st2)
                             && isnt_cyclic st1 && isnt_cyclic st2
                             && check_absence_vars_in_terms (get_Domain st1) (get_Images st2)
 
-(**States that if hd::tl and st2 are composable then tl and st2 are composable too**)
-val aux_lemma3 : hd:(variable*term) -> tl:subst -> st:subst -> Lemma
+(**States that if hd::tl and st are composable then tl and st are composable too**)
+val aux_lemma3a : hd:(variable*term) -> tl:subst -> st:subst -> Lemma
   (requires is_composable (hd::tl) st)
   (ensures is_composable tl st)
 
-let rec aux_lemma3 hd tl st = aux_lemma2 hd tl
+let rec aux_lemma3a hd tl st = aux_lemma2 hd tl
+
+val aux_lemma3b : #a:eqtype -> l1:list a -> hd:a -> tl:list a -> Lemma
+  (requires distinct_lists l1 (hd::tl))
+  (ensures distinct_lists l1 tl)
+
+let rec aux_lemma3b #a l1 hd tl = match l1 with
+  | [] -> ()
+  | xs::ys -> aux_lemma3b #a ys hd tl
+
+val aux_lemma3c : st1:subst -> hd:(variable*term) -> tl:subst -> Lemma
+  (requires distinct_domain st1 (hd::tl))
+  (ensures distinct_domain st1 tl)
+
+let aux_lemma3c st1 hd tl = aux_lemma3b (get_Domain st1) (fst hd) (get_Domain tl)
+
 
 (**Returns the composition of two substitutions**)
 val compose : st1:subst -> st2:subst -> Tot subst
@@ -150,7 +165,7 @@ val compose_aux_lemma1 : st1:subst -> st2:subst -> Lemma
 
 let rec compose_aux_lemma1 st1 st2 = match st1 with
   | [] -> ()
-  | hd::tl -> aux_lemma3 hd tl st2 ; compose_aux_lemma1 tl st2
+  | hd::tl -> aux_lemma3a hd tl st2 ; compose_aux_lemma1 tl st2
 
 (**Auxiliary lemma for compose_lemma.
   States that the term corresponding to a variable v in composition of st1 and st2 is
@@ -158,13 +173,13 @@ let rec compose_aux_lemma1 st1 st2 = match st1 with
   or the term in st2 itself which v corresponds to.  **)
 val compose_aux_lemma2 : st1:subst -> st2:subst -> x:variable -> Lemma
  (requires (is_composable st1 st2))
- (ensures ( (mem x (get_Domain st1) ==> mem x (get_Domain (compose st1 st2)) /\ (get_Term x (compose st1 st2) = apply st2 (get_Term x st1))) /\
-            (mem x (get_Domain st2) ==> mem x (get_Domain (compose st1 st2)) /\ (get_Term x (compose st1 st2) = get_Term x st2)) ) )
+ (ensures ( (mem x (get_Domain st1) ==> mem x (get_Domain (compose st1 st2)) /\ (get_Image x (compose st1 st2) = apply st2 (get_Image x st1))) /\
+            (mem x (get_Domain st2) ==> mem x (get_Domain (compose st1 st2)) /\ (get_Image x (compose st1 st2) = get_Image x st2)) ) )
 
 let rec compose_aux_lemma2 st1 st2 x = match st1 with
   | [] -> ()
   | hd::tl -> if x=fst hd then () else
-    (aux_lemma3 hd tl st2 ; compose_aux_lemma1 st1 st2; compose_aux_lemma2 tl st2 x)
+    (aux_lemma3a hd tl st2 ; compose_aux_lemma1 st1 st2; compose_aux_lemma2 tl st2 x)
 
 (**composition lemma.
   States that the application of composition of two substitutions is equal to
@@ -186,15 +201,20 @@ let rec compose_lemma st1 st2 t = match t with
   | [] -> ()
   | hd::tl -> compose_lemma st1 st2 hd ; compose_list_lemma st1 st2 tl
 
+
+(** States that if the variables in lv are not present in the list hd::tl then
+    they are neither present in the list [hd] nor in the list tl **)
 val aux_lemma4 : lv:list variable -> hd:term -> tl:list term -> Lemma
   (requires (check_absence_vars_in_terms lv (hd::tl)))
-  (ensures (check_absence_vars_in_terms lv (hd::[]) && (check_absence_vars_in_terms lv tl)))
+  (ensures (check_absence_vars_in_terms lv [hd] && (check_absence_vars_in_terms lv tl)))
   [SMTPat (check_absence_vars_in_terms lv (hd::tl))]
 
 let rec aux_lemma4 lv hd tl = match lv with
   | [] -> ()
   | xs::ys -> aux_lemma4 ys hd tl
 
+(** States that if the variables in the list lv are not present the term Func s args ,
+    then they are not present in any of the terms in the list args **)
 val aux_lemma5: t:term -> lv:list variable -> Lemma
   (requires ( check_absence_vars_in_terms lv [t]) )
   (ensures ( (Func? t) ==> (check_absence_vars_in_terms lv (Func?.l t)) ) )
@@ -203,6 +223,8 @@ let rec aux_lemma5 t lv = match lv with
   | [] -> ()
   | hd::tl -> aux_lemma5 t tl
 
+(** States that if the variables in the list lv are not present in the term Var v,
+    then v doesn't belong in the list lv **)
 val aux_lemma6 : lv:list variable -> t:term -> Lemma
   (requires check_absence_vars_in_terms lv [t] )
   (ensures ( (Var? t) ==> ( not(mem (Var?.v t) lv) ) ) )
@@ -211,6 +233,15 @@ let rec aux_lemma6 lv t = match lv with
   | [] -> ()
   | hd::tl -> aux_lemma6 tl t
 
+val aux_lemma7 : st:subst -> hd:(variable*term) -> tl:subst -> Lemma
+  (requires is_composable st (hd::tl))
+  (ensures is_composable st tl)
+
+let aux_lemma7 st hd tl =  aux_lemma2 hd tl; aux_lemma3c st hd tl; aux_lemma4 (get_Domain st) (snd hd) (get_Images tl)
+
+(** States that if vars(t) where t is a term is disjoint from Domain(st),
+    then application of st on t has no effect.
+    The corresponding lemma for lists follows.**)
 val commutation_aux_lemma1: t:term -> st:subst -> Lemma
   (requires (check_absence_vars_in_terms (get_Domain st) [t]) )
   (ensures (apply st t = t))
@@ -229,19 +260,31 @@ and commutation_aux_lemma1_list lt st= match lt with
               commutation_aux_lemma1 hd st ;
               commutation_aux_lemma1_list tl st
 
-val aux_lemma7: lv:list variable -> hd:list term -> tl:list term -> Lemma
+(** States that if the variables in the list lv are not present in the list hd::tl,
+  where hd and tl are both lists, then they are not present in tl either. **)
+val aux_lemma8: lv:list variable -> hd:list term -> tl:list term -> Lemma
   (requires check_absence_vars_in_terms lv (FStar.List.Tot.append hd tl))
   (ensures check_absence_vars_in_terms lv tl)
 
-let rec aux_lemma7 lv hd tl = match hd with
+let rec aux_lemma8 lv hd tl = match hd with
   | [] -> ()
-  | xs::ys -> aux_lemma4 lv xs (FStar.List.Tot.append ys tl) ; aux_lemma7 lv ys tl
+  | xs::ys -> aux_lemma4 lv xs (FStar.List.Tot.append ys tl) ; aux_lemma8 lv ys tl
 
+(** States that if the two substutions are mutually composable, then the domain of st2
+    is disjoint from the set vars(image of v in st1). **)
 val commutation_aux_lemma2: st1:subst -> st2:subst -> v:variable -> Lemma
   (requires (is_composable st1 st2 && is_composable st2 st1) )
-  (ensures (mem v (get_Domain st1) ==> check_absence_vars_in_terms (get_Domain st2) ((get_Term v st1)::[]) ))
+  (ensures (mem v (get_Domain st1) ==> check_absence_vars_in_terms (get_Domain st2) [get_Image v st1] ))
 
-let commutation_aux_lemma2 st1 st2 v = admit()
+let rec commutation_aux_lemma2 st1 st2 v =  match st1 with
+  | [] -> ()
+  | hd::tl -> if v=(fst hd) then ( assert (check_absence_vars_in_terms  (get_Domain st2) ((snd hd)::(get_Images tl)) ) )
+              else ( aux_lemma3a hd tl st2 ; aux_lemma7 st2 hd tl ; commutation_aux_lemma2 tl st2 v )
+  (*assert ( mem v (get_Domain st1) ==> (mem (get_Image v st1) (get_Images st1)) )*)
+
+(** Commutation lemma
+    States that if two substutions are mutually composable,
+    then the order of composition doesn't matter. **)
 
 val commutation_lemma : st1:subst -> st2:subst -> t:term-> Lemma
   (requires (is_composable st1 st2 && is_composable st2 st1) )
@@ -251,9 +294,10 @@ val commutation_list_lemma : st1:subst -> st2:subst -> lt:list term-> Lemma
   (requires (is_composable st1 st2 && is_composable st2 st1) )
   (ensures equal_subst_list (compose st1 st2) (compose st2 st1) lt)
 
-let rec commutation_lemma st1 st2 t = compose_lemma st1 st2 t; compose_lemma st2 st1 t; match t with
-  | Var v -> if mem v (get_Domain st1) then (commutation_aux_lemma2 st1 st2 v; commutation_aux_lemma1 (get_Term v st1) st2)
-             else if mem v (get_Domain st2) then (commutation_aux_lemma2 st2 st1 v; commutation_aux_lemma1 (get_Term v st2) st1)
+let rec commutation_lemma st1 st2 t = compose_aux_lemma1 st1 st2 ; compose_aux_lemma1 st2 st1 ;
+                                      compose_lemma st1 st2 t; compose_lemma st2 st1 t; match t with
+  | Var v -> if mem v (get_Domain st1) then (commutation_aux_lemma2 st1 st2 v; commutation_aux_lemma1 (get_Image v st1) st2)
+             else if mem v (get_Domain st2) then (commutation_aux_lemma2 st2 st1 v; commutation_aux_lemma1 (get_Image v st2) st1)
              else ()
   | Name n -> ()
   | Func s args -> commutation_list_lemma st1 st2 args
